WIP: fixed a typo in Globalenv.v

unusedglob/VerComp.v
@@ -408,514 +408,778 @@ Proof.
 Qed.
 *)
 
-(*
-(** * Test1: compose injp' ⋅ injp' = injp' *)
-
-(*
-L1 <=injp'->injp' L2 ->
-L2 <=injp'->injp' L3 ->
-L1 <= injp'-> injp' L3
-*)
 
 
+(** Pre: from cklr/CKLRAlgebra.v *)
 
+Definition subcklr' (Q R: cklr') :=
+  forall wq se1 se2 m1 m2,
+    match_stbls Q wq se1 se2 ->
+    match_mem Q wq m1 m2 ->
+    exists wr,
+      match_stbls R wr se1 se2 /\
+      match_mem R wr m1 m2 /\
+      inject_incr (mi Q wq) (mi R wr) /\
+      forall wr' m1' m2',
+        match_mem R wr' m1' m2' ->
+        wr ~> wr' ->
+        exists wq',
+          match_mem Q wq' m1' m2' /\
+          wq ~> wq' /\
+          inject_incr (mi R wr') (mi Q wq').
 
+Definition eqcklr' R1 R2 :=
+  subcklr' R1 R2 /\ subcklr' R2 R1.
 
-Section COMPOSE_FORWARD_SIMULATIONS.
-
-Context (L1: semantics li_c li_c) (L2: semantics li_c li_c) (L3: semantics li_c li_c).
-(*
-Definition symtbl_dom (se: Genv.symtbl) : meminj :=
-  fun b => if Mem.sup_dec b (Genv.genv_sup se) then Some (b,0)
-        else None.
-*)
-Definition source_inj (se: Genv.symtbl) (f : meminj) :=
-  fun b => if Mem.sup_dec b (Genv.genv_sup se) then
-        Some (b,0) else meminj_dom f b.
-
-Lemma source_inj_meminj_dom_incr : forall se f,
-    inject_incr (meminj_dom f) (source_inj se f).
+Global Instance subcklr_preo':
+  PreOrder subcklr'.
 Proof.
-  intros. intro. intros.
-  unfold source_inj.
-  unfold meminj_dom in *.
-  destruct (f b); try discriminate. inv H.
-  destruct Mem.sup_dec; eauto.
+  split.
+  - intros R w q1 q2 Hq.
+    exists w; intuition eauto.
+  - intros R1 R2 R3 H12 H23 w1 sea seb ma mb Hse1 Hm1.
+    destruct (H12 w1 sea seb ma mb Hse1 Hm1) as (w2 & Hse2 & Hm2 & Hincr12 & H21); clear H12.
+    destruct (H23 w2 sea seb ma mb Hse2 Hm2) as (w3 & Hse3 & Hm3 & Hincr23 & H32); clear H23.
+    exists w3. repeat apply conj; eauto using inject_incr_trans.
+    intros w3' ma' mb' Hm3' Hw3'.
+    destruct (H32 w3' ma' mb' Hm3' Hw3') as (w2' & Hm2' & Hw2' & Hincr32).
+    destruct (H21 w2' ma' mb' Hm2' Hw2') as (w1' & Hm1' & Hw1' & Hincr21).
+    exists w1'; intuition eauto using inject_incr_trans.
 Qed.
 
-Global Instance source_inj_incr se:
-  Monotonic (@source_inj se) (inject_incr ++> inject_incr).
+Global Instance eqcklr_equiv':
+  Equivalence eqcklr'.
 Proof.
-  intros f g Hfg b b' delta Hb.
-  unfold source_inj in *.
-  destruct (Mem.sup_dec). eauto.
-  eapply meminj_dom_incr; eauto.
+  split.
+  - intros R.
+    split; reflexivity.
+  - intros R1 R2. unfold eqcklr'.
+    tauto.
+  - intros R1 R2 R3 [H12 H21] [H23 H32].
+    split; etransitivity; eauto.
 Qed.
 
-Lemma source_inj_compose se f:
-  compose_meminj (source_inj se f) f = f.
+Global Instance subcklr_po':
+  PartialOrder eqcklr' subcklr'.
 Proof.
-  apply Axioms.functional_extensionality; intros b.
-  unfold compose_meminj, source_inj, meminj_dom.
-  destruct (Mem.sup_dec).
-  destruct (f b) as [[b' ofs] | ] eqn:Hfb; eauto.
-  destruct (f b) as [[b' ofs] | ] eqn:Hfb; eauto.
-  rewrite Hfb.
-  replace (0 + ofs) with ofs by extlia.
-  reflexivity.
+  unfold eqcklr'. red. generalize subcklr'.
+  firstorder.
 Qed.
 
-Lemma block_inject_dom se f b1 b2:
-  block_inject f b1 b2 ->
-  block_inject (source_inj se f) b1 b1.
+
+(** * Composition *)
+
+(** ** Definition *)
+
+(** ** Preliminaries *)
+
+Lemma option_le_compose {A B C} (R1: rel A B) (R2: rel B C):
+  eqrel
+    (option_le (rel_compose R1 R2))
+    (rel_compose (option_le R1) (option_le R2)).
 Proof.
-  unfold source_inj,meminj_dom.
-  intros (delta & Hb).
-  exists 0.
-  rewrite Hb; eauto.
-  destruct Mem.sup_dec; eauto.
+  split.
+  - intros _ _ [x z (y & Hxy & Hyz) | z];
+    eexists; split; constructor; eauto.
+  - intros x z (y & Hxy & Hyz).
+    destruct Hxy; [inversion Hyz; clear Hyz; subst | ];
+    constructor; eexists; split; eauto.
 Qed.
 
-Lemma val_inject_dom se f v1 v2:
-  Val.inject f v1 v2 ->
-  Val.inject (source_inj se f) v1 v1.
+Lemma list_rel_compose {A B C} (R1: rel A B) (R2: rel B C):
+  eqrel
+    (list_rel (rel_compose R1 R2))
+    (rel_compose (list_rel R1) (list_rel R2)).
 Proof.
-  destruct 1; econstructor.
-  - unfold source_inj, meminj_dom.
-    rewrite H. destruct Mem.sup_dec; eauto.
-  - rewrite Ptrofs.add_zero.
+  split.
+  - induction 1.
+    + exists nil; split; constructor.
+    + destruct H as (z & ? & ?).
+      destruct IHlist_rel as (z0 & ? & ?).
+      exists (z::z0); split; constructor; eauto.
+  - intros la lc (lb & H1 & H2).
+    revert lc H2.
+    induction H1; intros lc H2; inv H2.
+    + constructor.
+    + constructor; eauto.
+Qed.
+
+Global Instance compose_meminj_incr:
+  Monotonic compose_meminj (inject_incr ++> inject_incr ++> inject_incr).
+Proof.
+  intros f1 f2 Hf g1 g2 Hg b xb xdelta.
+  unfold compose_meminj.
+  destruct (f1 b) as [[b' delta] | ] eqn:Hb'; try discriminate.
+  erewrite Hf by eauto.
+  destruct (g1 b') as [[b'' delta'] | ] eqn:Hb''; try discriminate.
+  erewrite Hg by eauto.
+  tauto.
+Qed.
+
+Lemma val_inject_compose f g:
+  eqrel
+    (Val.inject (compose_meminj f g))
+    (rel_compose (Val.inject f) (Val.inject g)).
+Proof.
+  split.
+  - intros v1 v3 Hv.
+    destruct Hv; try (eexists; split; constructor).
+    unfold compose_meminj in H.
+    destruct (f b1) as [[bi di] | ] eqn:Hi; try discriminate.
+    destruct (g bi) as [[bj dj] | ] eqn:Hj; try discriminate.
+    inv H.
+    exists (Vptr bi (Ptrofs.add ofs1 (Ptrofs.repr di))).
+    split; econstructor; eauto.
+    rewrite add_repr, Ptrofs.add_assoc.
+    reflexivity.
+  - intros v1 v3 (v2 & Hv12 & Hv23).
+    destruct Hv12; inv Hv23; econstructor.
+    unfold compose_meminj.
+    + rewrite H, H3.
+      reflexivity.
+    + rewrite add_repr, Ptrofs.add_assoc.
+      reflexivity.
+Qed.
+
+Lemma memval_inject_compose f g:
+  eqrel
+    (memval_inject (compose_meminj f g))
+    (rel_compose (memval_inject f) (memval_inject g)).
+Proof.
+  split.
+  - intros v1 v3 Hv.
+    destruct Hv; try solve [eexists; split; constructor].
+    apply val_inject_compose in H.
+    destruct H as (vi & Hv1i & Hvi2).
+    eexists; split; constructor; eauto.
+  - intros v1 v3 Hv.
+    destruct Hv as (v2 & Hv12 & Hv23).
+    destruct Hv12; inv Hv23; constructor.
+    apply val_inject_compose.
+    eexists; split; eauto.
+Qed.
+
+Lemma ptr_inject_compose f g:
+  eqrel
+    (ptr_inject (compose_meminj f g))
+    (rel_compose (ptr_inject f) (ptr_inject g)).
+Proof.
+  split.
+  - intros v1 v3 Hv.
+    destruct Hv.
+    unfold compose_meminj in H.
+    destruct (f b1) as [[bi di] | ] eqn:Hi; try discriminate.
+    destruct (g bi) as [[bj dj] | ] eqn:Hj; try discriminate.
+    inv H.
+    rewrite Z.add_assoc.
+    exists (bi, ofs1 + di); split; econstructor; eauto.
+  - intros v1 v3 (v2 & Hv12 & Hv23).
+    destruct Hv12; inv Hv23.
+    rewrite <- Z.add_assoc.
+    constructor.
+    unfold compose_meminj.
+    rewrite H, H3.
     reflexivity.
 Qed.
 
-Lemma memval_inject_dom se f v1 v2:
-  memval_inject f v1 v2 ->
-  memval_inject (source_inj se f) v1 v1.
+Lemma ptrbits_inject_compose f g:
+  eqrel
+    (ptrbits_inject (compose_meminj f g))
+    (rel_compose (ptrbits_inject f) (ptrbits_inject g)).
 Proof.
-  destruct 1; econstructor.
-  eapply val_inject_dom; eauto.
+  split.
+  - destruct 1.
+    unfold compose_meminj in H.
+    destruct (f b1) as [[bI delta1I] | ] eqn:H1I; [ | discriminate].
+    exists (bI, Ptrofs.add ofs1 (Ptrofs.repr delta1I)); split; eauto.
+    destruct (g bI) as [[xb2 deltaI2] | ] eqn:HI2; [ | discriminate].
+    inv H.
+    rewrite add_repr.
+    rewrite <- Ptrofs.add_assoc.
+    constructor; eauto.
+  - intros p1 p3 (p2 & H12 & H23).
+    destruct H12 as [b1 ofs1 b2 delta12].
+    inv H23.
+    rewrite Ptrofs.add_assoc.
+    rewrite <- add_repr.
+    constructor.
+    unfold compose_meminj. rewrite H, H3.
+    reflexivity.
 Qed.
 
-Lemma val_inject_list_dom se f vs1 vs2:
-  Val.inject_list f vs1 vs2 ->
-  Val.inject_list (source_inj se f) vs1 vs1.
+Lemma rptr_inject_compose f g:
+  subrel
+    (rptr_inject (compose_meminj f g))
+    (rel_compose (rptr_inject f) (rptr_inject g)).
 Proof.
-  induction 1; constructor; eauto using val_inject_dom.
+  unfold rptr_inject.
+  intros p1 p3 Hp.
+  rewrite ptr_inject_compose in Hp.
+  rewrite ptrbits_inject_compose in Hp.
+  destruct Hp as [(p2 & H12 & H23) | [q1 q3 (q2 & H12 & H23)]].
+  - exists p2; split; rauto.
+  - exists (ptrbits_unsigned q2); split; rauto.
 Qed.
 
-Lemma global_blocks_pointer:
-  forall se m b ofs q n b' ofs',
-    Maps.ZMap.get ofs (NMap.get (Maps.ZMap.t memval) b (Mem.mem_contents m)) = (Fragment (Vptr b' ofs') q n) ->
-    sup_In b (Genv.genv_sup se) ->
-    sup_In b' (Genv.genv_sup se).
+Lemma ptrrange_inject_compose f g:
+  eqrel
+    (ptrrange_inject (compose_meminj f g))
+    (rel_compose (ptrrange_inject f) (ptrrange_inject g)).
 Proof.
+  split.
+  - destruct 1.
+    apply ptr_inject_compose in H.
+    destruct H as ([bi ofsi] & H1 & H2).
+    exists (bi, ofsi, ofsi + sz).
+    split; constructor; eauto.
+  - intros r1 r3 (r2 & H12 & H23).
+    destruct H12; inv H23.
+    assert (sz0 = sz) by lia; subst.
+    constructor.
+    apply ptr_inject_compose.
+    eexists; split; eauto.
+Qed.
+
+Lemma block_inject_compose f g:
+  eqrel
+    (block_inject (compose_meminj f g))
+    (rel_compose (block_inject f) (block_inject g)).
+Proof.
+  split.
+  - intros b1 b3 [d13 H13].
+    unfold compose_meminj in H13.
+    destruct (f b1) as [[b2 d12] | ] eqn:H12; [ | discriminate].
+    destruct (g b2) as [[xb3 d23] | ] eqn:H23; [ | discriminate].
+    inv H13.
+    exists b2; eexists; eauto.
+  - intros b1 b3 (b2 & [d2 H12] & [d3 H23]).
+    exists (d2 + d3).
+    unfold compose_meminj.
+    rewrite H12, H23.
+    reflexivity.
+Qed.
+
+Lemma block_inject_sameofs_compose f g:
+  subrel
+    (rel_compose (block_inject_sameofs f) (block_inject_sameofs g))
+    (block_inject_sameofs (compose_meminj f g)).
+Proof.
+  intros b1 b3 (b2 & H12 & H23).
+  red in H12, H23 |- *.
+  unfold compose_meminj. rewrite H12, H23.
+  reflexivity.
+Qed.
+
+Lemma flat_inj_idemp thr:
+  compose_meminj (Mem.flat_inj thr) (Mem.flat_inj thr) = Mem.flat_inj thr.
+Proof.
+  apply Axioms.functional_extensionality; intros b.
+  unfold compose_meminj, Mem.flat_inj.
+  destruct Mem.sup_dec eqn:Hb; eauto.
+  rewrite Hb.
+  reflexivity.
+Qed.
+
+Program Definition cklr_compose' (R1 R2: cklr'): cklr' :=
+  {|
+    world := world R1 * world R2;
+    wacc := wacc R1 * wacc R2;
+    mi w := compose_meminj (mi R1 (fst w)) (mi R2 (snd w));
+    match_stbls w := rel_compose (match_stbls R1 (fst w)) (match_stbls R2 (snd w));
+    match_mem w := rel_compose (match_mem R1 (fst w)) (match_mem R2 (snd w));
+  |}.
+
+Next Obligation.
+  rauto.
+Qed.
+
+(** mi_acc_separated *)
+Next Obligation.
+  rename w1 into w2'.
+  rename w0 into w1'.
+  rename w into w1.
+  intros b1 b2 delta Hw Hw'.
+
+  destruct H as (m & Hm1 & Hm2).
+  destruct H0 as [HR1 HR2].
+  cbn in *.
+
+  specialize (mi_acc_separated R1 _ _ _ _ Hm1 HR1) as sep1.
+  specialize (mi_acc_separated R2 _ _ _ _ Hm2 HR2) as sep2.
+  unfold inject_separated in sep1, sep2.
+  unfold compose_meminj in Hw, Hw'.
+  destruct (mi R1 w1' b1) as [[b11' delta11'] |] eqn:HR1w1'; [|discriminate].
+  destruct (mi R2 w2' b11') as [[b22' delta22'] |] eqn:HR2w2'; [|discriminate].
+  injection Hw'. clear Hw'. intros; subst delta b22'.
+  destruct (mi R1 w1 b1) as [[b11 delta11] |] eqn:HR1w1.
+  - destruct (mi R2 w2 b11) as [[b22 delta22] |] eqn:HR2w2.
+    discriminate.
+    assert (HR1w1'_alt: mi R1 w1' b1 = Some (b11, delta11)).
+    { eapply mi_acc; eauto. }
+    rewrite HR1w1' in HR1w1'_alt. inv HR1w1'_alt.
+    destruct (sep2 _ _ _ HR2w2 HR2w2') as [Hnvb11 Hnvb2].
+    split; [|assumption].
+    contradict Hnvb11.
+    eapply (cklr_valid_block _ _ _ _ Hm1); eauto.
+    eexists. eauto.
+  - destruct (sep1 _ _ _ HR1w1 HR1w1') as [Hnvb1 Hnvb11'].
+    split. auto.
+    destruct (mi R2 w2 b11') as [[b22 delta22] |] eqn:HR2w2.
+    + contradict Hnvb11'.
+      assert (HR2w2'_alt: mi R2 w2' b11' = Some (b22, delta22)).
+      { eapply mi_acc; eauto. }
+      rewrite HR2w2' in HR2w2'_alt. inv HR2w2'_alt.
+      eapply cklr_valid_block; eauto.
+      eexists. eauto.
+    + eapply sep2; eauto.
+Qed.
+
+Next Obligation.
+  intros [w12 w23] [w12' w23'] [H12 H23]. cbn.
+  eapply rel_compose_subrel; rauto.
+Qed.
+
+Next Obligation.
+  cbn. intros se1 se3 (se2 & Hse12 & Hse23).
+  apply match_stbls_proj in Hse12.
+  apply match_stbls_proj in Hse23.
+  eapply Genv.match_stbls'_compose; eauto.
+Qed.
+
+Next Obligation.
+  destruct H as (sei & Hse1i & Hsei2), H0 as (mi & Hm1i & Hmi2). cbn in *.
+  eapply (match_stbls_support R2); eauto.
+  eapply (match_stbls_support R1); eauto.
+Qed.
+
+Next Obligation.
+  intros [w12 w23] m1 m3 (m2 & Hm12 & Hm23) lo hi.
+  edestruct (cklr_alloc R1 w12 m1 m2 Hm12 lo hi)
+    as (w12' & Hw12' & Hm12' & Hb12).
+  edestruct (cklr_alloc R2 w23 m2 m3 Hm23 lo hi)
+    as (w23' & Hw23' & Hm23' & Hb23).
+  exists (w12', w23'); split; [rauto | ].
+  rstep. simpl. split.
+  - eexists; split; rauto.
+  - red. apply block_inject_sameofs_compose.
+    eexists; split; eauto.
+Qed.
+
+Next Obligation.
+  intros [w12 w23] m1 m3 (m2 & Hm12 & Hm23) [[b1 lo1] hi1] [[b3 lo3] hi3] H.
+  apply ptrrange_inject_compose in H.
+  destruct H as ([[b2 lo2] hi2] & Hr12 & Hr23).
+  simpl in *. red.
+  destruct (Mem.free m1 _ _ _) as [m1'|] eqn:H1; [|constructor].
+  (* transport H1.
+  transport H.
+  rewrite H1. constructor.
+  exists (w12', w23').
+  split; [rauto | ].
+  eexists; split; rauto. *)
 Admitted.
 
-Lemma mem_mem_inj_dom se f m1 m2:
-  Mem.mem_inj f m1 m2 ->
-  Mem.mem_inj (source_inj se f) m1 m1.
-Proof.
-  intros H.
-  split.
-  - unfold source_inj, meminj_dom. intros b1 b2 delta ofs k p Hb1 Hp.
-    destruct Mem.sup_dec; destruct (f b1); inv Hb1;
-    replace (ofs + 0) with ofs by extlia; auto.
-  - unfold source_inj, meminj_dom. intros b1 b2 delta chunk ofs p Hb1 Hrp.
-    destruct (Mem.sup_dec); destruct (f b1) as [[b1' delta'] | ]; inv Hb1;
-    eauto using Z.divide_0_r.
-  - unfold source_inj, meminj_dom at 1. intros b1 ofs b2 delta Hb1 Hp.
-    destruct (Mem.sup_dec) ; destruct (f b1) as [[b1' delta'] | ] eqn:Hb1'; inv Hb1.
-    replace (ofs + 0) with ofs by extlia.
-    eapply memval_inject_dom.
-    eapply Mem.mi_memval; eauto.
-    replace (ofs + 0) with ofs by extlia.
-    {
-      set (mv:= (Maps.ZMap.get ofs (NMap.get (Maps.ZMap.t memval) b2 (Mem.mem_contents m1)))).
-      destruct mv eqn:Hmem; constructor.
-      destruct v eqn:Hv; econstructor.
-      rewrite pred_dec_true. reflexivity.
-      eapply global_blocks_pointer; eauto.
-      rewrite Ptrofs.add_zero. reflexivity.
-    }
-    replace (ofs + 0) with ofs by extlia.
-    eapply memval_inject_dom.
-    eapply Mem.mi_memval; eauto.
+Next Obligation.
+  intros [w12 w23] chunk m1 m3 (m2 & Hm12 & Hm23) [b1 ofs1] [b3 ofs3] Hptr.
+  apply ptr_inject_compose in Hptr.
+  destruct Hptr as ([b2 ofs2] & Hptr12 & Hptr23).
+  red. simpl in *. unfold klr_pullw.
+  rewrite val_inject_compose.
+  apply option_le_compose.
+  eexists; split.
+Admitted.
+
+Next Obligation.
+  intros [w12 w23] chunk m1 m3 (m2 & Hm12 & Hm23) [b1 o1] [b3 o3] Hptr v1 v3 Hv.
+  simpl in *. red. unfold klr_pullw in *.
+  apply ptr_inject_compose in Hptr. destruct Hptr as ([b2 o2] & Hp12 & Hp23).
+  apply val_inject_compose in Hv. destruct Hv as (v2 & Hv12 & Hv23).
+  destruct (Mem.store chunk m1 b1 o1 v1) as [m1'|] eqn:H1; [|constructor].
+(*
+  transport H1.
+  transport H.
+  rewrite H1. constructor.
+  exists (w12', w23'); split; [rauto | ].
+  eexists; split; try rauto.
+Qed.
+ *)
+Admitted.
+
+Next Obligation.
+  intros [w12 w23] m1 m3 (m2 & Hm12 & Hm23) [b1 ofs1] [b3 ofs3] Hptr sz.
+  apply ptr_inject_compose in Hptr.
+  destruct Hptr as ([b2 ofs2] & Hptr12 & Hptr23).
+  unfold k1, klr_pullw. simpl in *.
+  eapply option_le_subrel. (* XXX coqrel *)
+  {
+    apply list_subrel.
+    apply memval_inject_compose.
+  }
+  rewrite list_rel_compose.
+  apply option_le_compose.
+Admitted.
+(*
+  eexists; split; rauto.
+Qed.
+ *)
+
+Next Obligation.
+  intros [w12 w23] m1 m3 (m2 & Hm12 & Hm23) [b1 o1] [b3 o3] Hptr v1 v3 Hv.
+  unfold k1, klr_pullw in *. simpl in *.
+  apply rptr_inject_compose in Hptr. destruct Hptr as ([b2 o2] & Hp12 & Hp23).
+  rewrite memval_inject_compose in Hv. apply list_rel_compose in Hv.
+  destruct Hv as (v2 & Hv12 & Hv23).
+  destruct (Mem.storebytes m1 b1 o1 v1) as [m1'|] eqn:H1; [|constructor].
+  transport H1.
+  transport H.
+  rewrite H1. constructor.
+  exists (w12', w23'); split; [rauto | ].
+  eexists; split; try rauto.
 Qed.
 
-Lemma mem_source_inj se f m1 m2:
-  Mem.sup_include (Genv.genv_sup se) (Mem.support m1) ->
-  Mem.inject f m1 m2 ->
-  Mem.inject (source_inj se f) m1 m1.
-Proof.
-  intros H.
-  split.
-  - eapply mem_mem_inj_dom.
-    eapply Mem.mi_inj; eauto.
-  - unfold source_inj, meminj_dom. intros.
-    erewrite Mem.mi_freeblocks; eauto.
-    rewrite pred_dec_false; eauto.
-    intro. apply H1. apply H. eauto.
-  - unfold source_inj, meminj_dom; intros.
-    destruct Mem.sup_dec; eauto. inv H1. apply H; eauto.
-    destruct (f b) as [[b'' delta'] | ] eqn:Hb; inv H1.
-    eapply Mem.valid_block_inject_1; eauto.
-  - red. unfold source_inj, meminj_dom. intros.
-    destruct Mem.sup_dec; inv H2; eauto.
-    destruct Mem.sup_dec; inv H3; eauto.
-    destruct (f b2); inv H6; eauto.
-    destruct Mem.sup_dec; inv H3; eauto.
-    destruct (f b1); inv H7; eauto.                              
-    destruct (f b1); inv H7.
-    destruct (f b2); inv H6.
+Next Obligation.
+  intros [w12 w23] m1 m3 Hm [b1 o1] [b3 o3] Hptr pk pe.
+  unfold k, klr_pullw in *. simpl in *.
+  destruct Hm as (m2 & Hm12 & Hm23).
+  apply ptr_inject_compose in Hptr. destruct Hptr as ([b2 o2] & Hp12 & Hp23).
+  etransitivity. instantiate (1:= Mem.perm m2 b2 o2 pk pe).
+  generalize (cklr_perm R1). intro. rauto.
+  generalize (cklr_perm R2). intro. rauto.
+Qed.
+
+Next Obligation.
+  intros [w12 w23] m1 m3 Hm b1 b3 Hb.
+  unfold k, klr_pullw in *. simpl in *.
+  destruct Hm as (m2 & Hm12 & Hm23).
+  apply block_inject_compose in Hb. destruct Hb as (b2 & Hb12 & Hb23).
+  etransitivity; rauto.
+Qed.
+
+Next Obligation. (* no overlap *)
+  intros a1 a2 da b1 b2 db oa ob Hab1 Ha Hb Hoa Hob. simpl in *.
+  destruct H as (mx & Hm1x & Hmx2).
+  unfold compose_meminj in *.
+  destruct (mi R1 w a1) as [[ax da1x] | ] eqn:Ha1x; [ | discriminate].
+  destruct (mi R2 w0 ax) as [[ay dax2] | ] eqn:Hax2; [ | discriminate].
+  inv Ha.
+  destruct (mi R1 w b1) as [[bx db1x] | ] eqn:Hb1x; [ | discriminate].
+  destruct (mi R2 w0 bx) as [[bz dbz2] | ] eqn:Hbx2; [ | discriminate].
+  inv Hb.
+  assert (Mem.perm mx ax (oa + da1x) Max Nonempty).
+  { revert Hoa. generalize (cklr_perm R1). intro. repeat rstep. constructor. eauto. }
+  assert (Mem.perm mx bx (ob + db1x) Max Nonempty).
+  { revert Hob. generalize (cklr_perm R1). intro. repeat rstep. constructor; eauto. }
+  edestruct (cklr_no_overlap R1 w m1 mx); eauto.
+  - edestruct (cklr_no_overlap R2 w0 mx m2); eauto.
+    rewrite !Z.add_assoc.
     eauto.
-  - unfold source_inj, meminj_dom. intros.
-    destruct (Mem.sup_dec); eauto. inv H1.
-    split; try extlia. rewrite Z.add_0_r.
-    apply Ptrofs.unsigned_range_2.
-    destruct (f b); inv H1.
-    split; try extlia.
-    rewrite Z.add_0_r.
-    apply Ptrofs.unsigned_range_2.
-  - unfold source_inj, meminj_dom. intros.
-    destruct Mem.sup_dec; inv H1.
-    rewrite Z.add_0_r in H2; eauto.
-    destruct (f b1); inv H4.
-    rewrite Z.add_0_r in H2; eauto.
+  - destruct (eq_block ax bx); eauto.
+    + right. assert (dax2 = dbz2) by congruence. extlia.
+    + edestruct (cklr_no_overlap R2 w0 mx m2); eauto.
+      rewrite !Z.add_assoc.
+      eauto.
 Qed.
 
-Lemma match_stbls'_dom f se1 se2:
-  Genv.match_stbls' f se1 se2 ->
-  Genv.match_stbls' (source_inj se1 f) se1 se1.
-Proof.
-  intros Hse. unfold source_inj, meminj_dom. split; eauto; intros.
-  - rewrite pred_dec_true in H0; eauto. inv H0. reflexivity.
-  - eexists. rewrite pred_dec_true; eauto.
-  - destruct (Mem.sup_dec); eauto; inv H. reflexivity.
-    destruct (f b1) as [[xb2 xdelta] | ] eqn:Hb; inv H1. reflexivity.
-  - destruct (Mem.sup_dec); eauto; inv H. reflexivity.
-    destruct (f b1) as [[xb2 xdelta] | ] eqn:Hb; inv H1. reflexivity.
-  - destruct (Mem.sup_dec); eauto; inv H. reflexivity.
-    destruct (f b1) as [[xb2 xdelta] | ] eqn:Hb; inv H1. reflexivity.
+Next Obligation. (* representable *)
+  destruct H as (mI & Hm1I & HmI2).
+  unfold compose_meminj in H1. simpl in H1.
+  destruct (mi R1 w b1) as [[bI d1I] | ] eqn:H1I; [ | discriminate].
+  destruct (mi R2 w0 bI) as [[xb2 dI2] | ] eqn:HI2; [ | discriminate].
+  inv H1.
+  simpl in *.
+  assert (d1I >= 0 /\ 0 <= ofs1 + d1I <= Ptrofs.max_unsigned) as [? ?].
+  { eapply (cklr_representable R1); eauto. }
+  assert (dI2 >= 0 /\ 0 <= (ofs1 + d1I) + dI2 <= Ptrofs.max_unsigned).
+  { eapply (cklr_representable R2); eauto.
+    revert H0. generalize (cklr_perm R1). intro.
+    repeat rstep.
+    - constructor; eauto.
+    - replace (ofs1 + d1I -1) with (ofs1 - 1 + d1I) by extlia.
+      constructor; eauto. }
+  extlia.
 Qed.
 
-Lemma loc_unmapped_dom f b ofs:
-  loc_unmapped (meminj_dom f) b ofs <->
-  loc_unmapped f b ofs.
-Proof.
-  unfold meminj_dom, loc_unmapped.
-  destruct (f b) as [[b' delta] | ].
-  - split; discriminate.
-  - reflexivity.
-Qed.
-
-Definition source_world f m1 m2 (Hm: Mem.inject f m1 m2) (se:Genv.symtbl) (Hse: Mem.sup_include (Genv.genv_sup se) (Mem.support m1)) :=
-     injpw (source_inj se f) m1 m1 (mem_source_inj se f m1 m2 Hse Hm).
-
-Lemma match_stbls_dom' f se1 se2:
-  Genv.match_stbls' f se1 se2 ->
-  Genv.match_stbls (source_inj se1 f) se1 se1.
-Proof.
-  intros Hse. unfold source_inj. unfold meminj_dom. split; eauto; intros.
-  - destruct Mem.sup_dec; try congruence. eauto.
-  - inv Hse. exists b2. destruct Mem.sup_dec; try congruence.
-  - destruct Mem.sup_dec. inv H. reflexivity.
-    destruct (f b1) as [[xb2 xdelta] | ] eqn:Hb; inv H. reflexivity.
-  - destruct Mem.sup_dec. inv H. reflexivity.
-    destruct (f b1) as [[xb2 xdelta] | ] eqn:Hb; inv H. reflexivity.
-  - destruct Mem.sup_dec. inv H. reflexivity.
-    destruct (f b1) as [[xb2 xdelta] | ] eqn:Hb; inv H. reflexivity.
-Qed.
-
-Lemma compose_meminj_midvalue: forall j1 j2 v1 v3,
-    Val.inject (compose_meminj j1 j2) v1 v3 ->
-    exists v2, Val.inject j1 v1 v2 /\ Val.inject j2 v2 v3.
-Proof.
-  intros. inv H.
-  eexists. split; econstructor; eauto.
-  eexists. split; econstructor; eauto.
-  eexists. split; econstructor; eauto.
-  eexists. split; econstructor; eauto.
-  unfold compose_meminj in H0.
-  destruct (j1 b1) as [[b2' d1]|] eqn:M1; try congruence.
-  destruct (j2 b2') as [[b3' d2]|] eqn:M2; inv H0.
-  eexists. split. econstructor; eauto.
-  econstructor; eauto. rewrite add_repr.
-  rewrite Ptrofs.add_assoc. auto.
-  exists Vundef. split; constructor.
-Qed.
-
-
-Lemma compose_fsim_components_old_new:
-  fsim_components (cc_c injp) (cc_c injp) L1 L2 ->
-  fsim_components' (cc_c' injp') (cc_c' injp') L2 L3 ->
-  fsim_components' (cc_c' injp') (cc_c' injp') L1 L3.
-  intros [index order match_states Hsk props order_wf].
-  intros [index' order' match_states' Hsk' props' order_wf'].
-  set (ff_index := (index' * index)%type).
-  set (ff_order := lex_ord (clos_trans _ order') order).
-  set (ff_match_states :=
-         fun se1 se3 (w: injp_world) (i: ff_index) (s1: state L1) (s3: state L3) =>
-           exists s2 w12 w23,
-             match_states se1 se1 w12 (snd i) s1 s2 /\
-             match_states' se1 se3 w23 (fst i) s2 s3 /\
-               match_senv (cc_c injp) w12 se1 se1 /\
-               match_senv' (cc_c' injp') w23 se1 se3 /\
-               forall r1 r2 r3, match_reply (cc_c injp) w12 r1 r2 /\
-                             match_reply' (cc_c' injp') w23 r2 r3 ->
-                           match_reply' (cc_c' injp') w r1 r3).
-  apply Forward_simulation' with ff_order ff_match_states.
-  3: { unfold ff_order. auto using wf_lex_ord, wf_clos_trans. }
-  1: { congruence. }
-  intros se1 se2 w Hse2 Hcompat. cbn in *.
-  destruct w as [j m1 m2 Hm]. inversion Hse2. subst.
-  set (w1 := source_world j m1 m2 Hm se1 H5).
-  assert (Hse1: injp_match_stbls w1 se1 se1).
-  { constructor; eauto.
-    eapply  match_stbls_dom'; eauto.
-  }
-  assert (Hvalid1: Genv.valid_for (skel L1) se1).
-  {
-    inv Hcompat. eauto.
-  }
-  rewrite Hsk in Hcompat.
-  (* exploit props; eauto. intros Fsim1.*)
-  (* exploit props'; eauto. intros Fsim2. *)
-  split.
-- (* valid query *)
-  intros q1 q3 Hq13.
-  assert (match_query (cc_c injp) w1 q1 q1).
-  {
-    unfold w1. inv Hq13. cbn in *. inv H1. constructor; cbn in *.
-    eapply val_inject_dom; eauto.
-    eapply val_inject_list_dom; eauto.
-    econstructor; eauto. eauto.
-  }
-  etransitivity.
-  eapply fsim_match_valid_query'; eauto.
-  eapply fsim_match_valid_query; eauto.
-- (* initial states *)
-  intros q1 q3 s1 Hq13 Hs1.
-  assert (match_query (cc_c injp) w1 q1 q1).
-  {
-    unfold w1. inv Hq13. cbn in *. inv H1. constructor; cbn in *.
-    eapply val_inject_dom; eauto.
-    eapply val_inject_list_dom; eauto.
-    econstructor; eauto. eauto.
-  }
-  edestruct (@fsim_match_initial_states) as (i & s2 & A & B); eauto.
-  edestruct (@fsim_match_initial_states') as (i' & s3 & C & D); eauto.
-  exists (i', i); exists s3; split; auto. exists s2.
-  exists w1,(injpw j m1 m2 Hm). repeat apply conj; cbn; eauto.
-  intros r1 r2 r3 [[w1' [Hw1 Hr1]] [w2' [Hw2 Hr2]]].
-  destruct w1' as [j12' m1' m2' Hm12'].
-  destruct w2' as [j23' m2'x m3' Hm23'].
-  inv Hr1. inv Hr2. cbn in *. inv H1.  inv H9.
-  rename m1'0 into m1'. rename m2'0 into m2'. rename m2'1 into m3'.
-  exists (injpw (compose_meminj j12' j23') m1' m3' (Mem.inject_compose j12' j23' _ _ _ Hm12' Hm23')). repeat apply conj.
-  +  (*injp acc*)
-    unfold w1 in Hw1. inv Hw1. inv Hw2.
+Next Obligation. (* aligned_area_inject *)
+  destruct H as (mI & Hm1I & HmI2).
+  unfold compose_meminj in H5. simpl in H5.
+  destruct (mi R1 w b) as [[bI d1I] | ] eqn:H1I; [ | discriminate].
+  destruct (mi R2 w0 bI) as [[xb2 dI2] | ] eqn:HI2; [ | discriminate].
+  inv H5.
+  simpl in *.
+  rewrite Z.add_assoc.
+  eapply (cklr_aligned_area_inject R2); eauto.
+  - intros x Hx.
+    assert (Mem.perm m b (x - d1I) Cur Nonempty). { eapply H3. extlia. }
+    revert H. generalize (cklr_perm R1). intro. repeat rstep.
+    replace x with (x - d1I + d1I) at 2 by extlia.
     constructor; eauto.
-    -- (* m1 - unmapped *)
-      admit. (*TODO here: *)
-    -- (*inject_incr*)
-      rewrite <- source_inj_compose with (se := se1) (f := j).
-      rauto.
-    -- (*prove that the mapping we added to j12 does not involve j13 and j13'*)
-      intros b1 b2 delta Hb Hb'. unfold compose_meminj in Hb'.
-      destruct (j12' b1) as [[bi delta12] | ] eqn:Hb1; try discriminate.
-        destruct (j23' bi) as [[xb2 delta23] | ] eqn:Hb2; try discriminate.
+  - eapply (cklr_aligned_area_inject R1); eauto.
+Qed.
+
+Next Obligation. (* disjoint_or_equal_inject *)
+  simpl in *.
+  destruct H as (mI & Hm1I & HmI2).
+  unfold compose_meminj in *.
+  destruct (mi R1 w b1) as [[b1I d1] | ] eqn:Hb1I; [ | discriminate].
+  destruct (mi R2 w0 b1I) as [[xb1' d1'] | ] eqn:Hb1'; [ | discriminate].
+  inv H0.
+  destruct (mi R1 w b2) as [[b2I d2] | ] eqn:Hb2I; [ | discriminate].
+  destruct (mi R2 w0 b2I) as [[xb2' d2'] | ] eqn:Hb2'; [ | discriminate].
+  inv H1.
+  rewrite !Z.add_assoc.
+  eapply (cklr_disjoint_or_equal_inject R2); eauto.
+  - intros x Hx.
+    assert (Mem.perm m b1 (x - d1) Max Nonempty). { eapply H2. extlia. }
+    revert H. generalize (cklr_perm R1). intro. repeat rstep.  
+    replace x with (x - d1 + d1) at 2 by extlia.
+    constructor; eauto.
+  - intros x Hx.
+    assert (Mem.perm m b2 (x - d2) Max Nonempty). { eapply H3. extlia. }
+    revert H. generalize (cklr_perm R1). intro. repeat rstep.
+    replace x with (x - d2 + d2) at 2 by extlia.
+    constructor; eauto.
+  - eapply (cklr_disjoint_or_equal_inject R1); eauto.
+Qed.
+
+Next Obligation. (* perm inv *)
+  simpl in *.
+  destruct H as (mi & Hm1i & Hmi2).
+  apply ptr_inject_compose in H0 as ([bi ofsi] & Hp1i & Hpi2).
+  edestruct (cklr_perm_inv R2); eauto.
+  - eapply (cklr_perm_inv R1); eauto.
+  - right. intros Hm1. apply H. revert Hm1. generalize (cklr_perm R1). intro. rauto.
+Qed.
+
+
+Next Obligation. (* sup include *)
+  destruct H as (mI & Hm1I & Hm2I).
+  destruct H0 as ([w' w0'] & Hw' & mI' & Hm1I' & Hm2I').
+  cbn [fst snd] in *. unfold Ple in *.
+  inv Hw'; cbn in *.
+  etransitivity; eapply cklr_sup_include; eauto; eexists; split; eauto.
+Qed.
+
+Declare Scope cklr_scope.
+Bind Scope cklr_scope with cklr.
+Delimit Scope cklr_scope with cklr.
+Infix "#" := cklr_compose' (at level 30, right associativity) : cklr_scope.
+
+(** ** Properties *)
+
+(** Monotonicity *)
+
+Global Instance cklr_compose_subcklr:
+  Proper (subcklr ++> subcklr ++> subcklr) (@cklr_compose).
+Proof.
+  intros R12 R12' H12 R23 R23' H23.
+  intros [w12 w23] se1 se3 m1 m3 (se2 & Hse12 & Hse23) (m2 & Hm12 & Hm23). simpl in *.
+  specialize (H12 w12 se1 se2 m1 m2 Hse12 Hm12) as (w12' & Hse12' & Hm12' & Hincr12 & H12).
+  specialize (H23 w23 se2 se3 m2 m3 Hse23 Hm23) as (w23' & Hse23' & Hm23' & Hincr23 & H23).
+  exists (w12', w23'); simpl.
+  repeat apply conj; try rauto.
+  - eexists; split; eauto.
+  - eexists; split; eauto.
+  - intros [v12' v23'] m1' m3' (m2' & Hm'12 & Hm'23) [Hwv12 Hwv23].
+    specialize (H12 v12' m1' m2' Hm'12 Hwv12) as (v12 & Hm'12' & Hwv12' & Hi12').
+    specialize (H23 v23' m2' m3' Hm'23 Hwv23) as (v23 & Hm'23' & Hwv23' & Hi23').
+    simpl in *.
+    exists (v12, v23).
+    split; [ | split].
+    + eexists; split; eauto.
+    + rauto.
+    + rauto.
+Qed.
+
+(*
+(** Associativity *)
+
+Require Import Axioms.
+Lemma cklr_compose_assoc R1 R2 R3:
+  subcklr ((R1 @ R2) @ R3) (R1 @ (R2 @ R3)).
+Proof.
+  intros [[w1 w2] w3] sea sed ma md (seb & (sec & Hse1 & Hse2) & Hse3) (mb & (mc & Hm1 & Hm2) & Hm3).
+  simpl in *.
+  exists (w1, (w2, w3)).
+  repeat apply conj.
+  - repeat (eexists; eauto).
+  - repeat (eexists; eauto).
+  - rewrite compose_meminj_assoc. apply inject_incr_refl.
+  - intros (w1' & w2' & w3') ma' md' (mb' & Hm1' & (mc' & Hm2' & Hm3')).
+    intros (Hw1 & Hw2 & Hw3).
+    simpl in *.
+    exists ((w1', w2'), w3').
+    split; [ | split].
+    + repeat (econstructor; eauto).
+    + rauto.
+    + rewrite compose_meminj_assoc. apply inject_incr_refl.
+Qed.
+*)
+
+(** * Properties of [cc_c] *)
+
+Global Instance cc_c_ref':
+  Monotonic (@cc_c') (subcklr' ++> ccref').
+Proof.
+  intros Q R HQR. red in HQR |- *.
+  intros w se1 se2 q1 q2 Hse Hq.
+  destruct Hq as [vf1 vf2 sg vargs1 vargs2 m1 m2 Hvf Hvargs Hm].
+  specialize (HQR w se1 se2 m1 m2 Hse Hm) as (wr & HseR & HmR & Hincr & HQR').
+  exists wr. simpl in *. repeat apply conj; auto.
+  - constructor; eauto.
+  - intros r1 r2 (wr' & Hw' & Hr). destruct Hr as [v1 v2 m1' m2' Hvres Hm'].
+    specialize (HQR' wr' m1' m2' Hm' Hw') as (w' & HmQ' & HwQ' & Hincr').
+    eexists. split; eauto. constructor; eauto.
+Qed.
+
+Lemma match_c_query_compose R12 R23 w12 w23:
+  eqrel
+    (cc_c_query' (cklr_compose' R12 R23) (w12, w23))
+    (rel_compose (cc_c_query' R12 w12) (cc_c_query' R23 w23)).
+Proof.
+  split.
+  - intros _ _ [vf1 vf3 sg vargs1 vargs3 m1 m3 Hvf Hvargs Hm].
+    simpl in *.
+    apply val_inject_compose in Hvf. destruct Hvf as (vf2 & Hvf12 & Hv23).
+    apply val_inject_list_compose in Hvargs. destruct Hvargs as (vargs2 & ? & ?).
+    destruct Hm as (m2 & Hm12 & Hm23).
+    exists (cq vf2 sg vargs2 m2); split; constructor; simpl; eauto.
+    destruct Hvf12; congruence.
+  - intros q1 q3 (q2 & Hq12 & Hq23).
+    destruct Hq23 as [vf1 vf2 sg vargs2 vargs3 m2 m3 Hvf Hvargs23 Hm23 Hvf1].
+    inv Hq12.
+    constructor; simpl.
+    + apply val_inject_compose. ercompose; eauto.
+    + apply val_inject_list_compose. ercompose; eauto.
+    + ercompose; eauto.
+    + auto.
+Qed.
+(*
+Lemma cc_c_compose R12 R23:
+  cceqv' (cc_c' (R12 R23)) (cklr_compose' (cc_c' R12) (cc_c' R23)).
+Proof.
+  split.
+  - intros [w12 w23] se1 se3 q1 q3 (se2 & Hse12 & Hse23) Hq.
+    apply match_c_query_compose in Hq as (q2 & Hq12 & Hq23).
+    exists (se2, w12, w23).
+    repeat apply conj; cbn; eauto.
+    intros r1 r3 (r2 & (w12' & Hw21' & Hr12) & (w23' & Hw23' & Hr23)).
+    exists (w12', w23'). split. constructor; cbn; auto.
+    destruct Hr12; inv Hr23.
+    constructor; cbn; eauto.
+    apply val_inject_compose; eauto.
+  - intros [[se2 w12] w23] se1 se3 q1 q3 (Hse12 & Hse23) (q2 & Hq12 & Hq23).
+    cbn in *. exists (w12, w23). repeat apply conj; eauto.
+    + apply match_c_query_compose; eauto.
+    + intros r1 r3 ([w12' w23'] & Hw' & Hr).
+      destruct Hr. cbn in *.
+      apply val_inject_compose in H.
+      destruct Hw' as [? ?], H as (vi & ? & ?), H0 as (mi & ? & ?).
+      exists (cr vi mi).
+      split; eexists; constructor; eauto; constructor; eauto.
+Qed.
+ *)
+
+(** * easy part : compose injp' ⋅ injp ≡ injp' *)
+
+(* Maybe we can trans cklr into cklr'. Or we can have a more clean solution later *)
+(*
+Definition callconv_gen (R : cklr) : cklr' :=
+  {|
+    world := CKLR.world R;
+    wacc := CKLR.wacc R;
+    mi w := (CKLR.mi R) w;
+    match_stbls w := (CKLR.match_stbls R) w;
+    match_mem w := (CKLR.match_mem R) w;
+  |}.
+*)
+  
+
+Theorem injp'_injp_ref1:
+  ccref'  (cc_c' injp') (cc_compose_2 (cc_c' injp') (cc_c injp)).
+Proof.
+  red. intros w se1 se2 q1 q2 Hse Hq.
+  inv Hse. inv Hq. cbn in H2, H3. inv H4. rename m0 into m1. rename m3 into m2.
+  exists (se1, (injpw (meminj_dom f) (Genv.genv_sup se1) (Genv.genv_sup se1) m1 m1 (mem_inject_dom f m1 m2 Hm)),
+      (injpw f (Genv.genv_sup se1) (Genv.genv_sup se2) m1 m2 Hm)).
+  repeat apply conj.
+  - constructor.
+    (* problem here... we need to construct a reduced se1? *)
+    admit.
+    admit.
+  - exists (cq vf1 sg vargs1 m1). split.
+    econstructor; cbn; eauto.
+    eapply val_inject_dom; eauto.
+    eapply val_inject_list_dom; eauto.
+    constructor; cbn; eauto.
+  - intros r1 r3 [r2 [Hr1 Hr2]].
+    destruct Hr1 as [w12' [Hw12 Hr1]]. destruct Hr2 as [w23' [Hw23 Hr2]].
+    destruct w12' as [f12' ? ? m1' m2' Hm12']. destruct w23' as [f23' ? ? m2'' m3' Hm23'].
+    inv Hw12. inv Hw23. cbn in *.
+    inv Hr1. inv Hr2. cbn in *. inv H6. inv H11.
+    rename m1'0 into m1'. rename m2'0 into m2'. rename m2'1 into m3'.
+    eexists (injpw (compose_meminj f12' f23') (Genv.genv_sup se1) (Genv.genv_sup se2) m1' m3'
+               (Mem.inject_compose f12' f23' _ _ _ Hm12' Hm23')
+            ).
+    repeat apply conj.
+    + constructor; eauto.
+      * eapply Mem.unchanged_on_implies; eauto.
+        intros. destruct H6. split. red. unfold meminj_dom. rewrite H6. reflexivity. eauto.
+      * red. intros. unfold compose_meminj.
+        erewrite H21. erewrite H29; eauto.
+        2: unfold meminj_dom; rewrite H6; reflexivity.
+        rewrite Z.add_0_l. reflexivity.
+      * intros b1 b2 delta Hb Hb'. unfold compose_meminj in Hb'.
+        destruct (f12' b1) as [[bi delta12] | ] eqn:Hb1; try discriminate.
+        destruct (f23' bi) as [[xb2 delta23] | ] eqn:Hb2; try discriminate.
         inv Hb'.
-        edestruct H18; eauto.
-        unfold source_inj. destruct Mem.sup_dec.
-      ++ (*b1 is added as static variables which are removed from L2 to L3*)
-        (*we show that the same block bi for same variable is unmapped in j23 and j23'*)
-        assert ((source_inj se1 j) b1 = Some (b1,0)).
-        unfold source_inj. rewrite pred_dec_true. eauto. eauto.
-        erewrite H17 in Hb1; eauto. inv Hb1.
-        exploit H26; eauto. intros [E F].
-        clear - Hse1 E s.
-        unfold w1 in Hse1. inv Hse1.
-        exfalso. eapply E. eapply H6. eauto.
-      ++ unfold meminj_dom. rewrite Hb. auto.
-      ++ 
-        destruct (j bi) as [[? ?] | ] eqn:Hfbi.
+        edestruct H22; eauto. unfold meminj_dom. rewrite Hb. auto.
+        destruct (f bi) as [[? ?] | ] eqn:Hfbi.
         {
           eapply Mem.valid_block_inject_1 in Hfbi; eauto.
         }
-        edestruct H26; eauto.
-  + econstructor; cbn ; eauto. eapply val_inject_compose; eauto.
-- (* final states *)
-  intros. destruct H as (s3 & w12 & w23 & A & B & C & D & E).
-  edestruct (@fsim_match_final_states) as (r2 & Hr2 & Hr12); eauto.
-  edestruct (@fsim_match_final_states') as (r3 & Hr3 & Hr23); eauto.
-  exists r3. split. eauto. eapply E. split. eapply Hr12. eauto.
-- (* external states *)
-  intros. destruct H as (s3 & w12 & w23 & A & B & C & D & E).
-  edestruct (@fsim_match_external) as (w12A & q2 & Hq2 & Hq12 & Hw12 & Hk12); eauto.
-  edestruct (@fsim_match_external') as (w23A & q3 & Hq3 & Hq23 & Hw23 & Hk23); eauto.
-  {
-    cbn in *. destruct w12A as [j12 m1' m2' Hm12'].
-    inv Hq12. cbn in *. inv H3. rename m0 into m1'. rename m3 into m2'.
-    destruct w23A as [j23 m2'' m3' Hm23'].
-    inv Hq23. cbn in *. inv H13. rename m3 into m3'.
-    exists (injpw (compose_meminj j12 j23) m1' m3' (Mem.inject_compose _ _ _ _ _ Hm4 Hm7)).
-    exists (cq vf3 sg vargs3 m3').
-    repeat apply conj; eauto.
-    - (*match_query*)
-      econstructor; cbn; eauto. eapply val_inject_compose; eauto.
-      eapply val_inject_list_compose; eauto.
-    - (*match_stbls'*)
-      clear - Hw23 Hw12. cbn in *. inv Hw12. inv Hw23.
-      constructor; eauto.
-      eapply Genv.match_stbls_stbls'_compose; eauto.
-    - (*after_external*)
-      cbn.
-      intros r1 r3 s1' [w13' [Hw Hr13]] Hafter.
-      inv Hr13. inv H7. cbn in *. rename f into j13'. rename Hm11 into INJ13'.
-      cbn in Hw. rename m1'0 into m1'A. rename m2'0 into m3'A.
-      rename m1' into m1A. rename m2' into m2A. rename m3' into m3A.
-      rename Hm4 into INJ12. rename Hm7 into INJ23.
-      inversion Hw as [? ? ? ? ? ? ? ? RO1 RO3 MAXPERM1 MAXPERM3 UNCHANGE1 UNCHANGE3 INCR13 DISJ13]. subst.
-      generalize (inject_implies_image_in _ _ _ INJ12).
-      intros IMGIN12.
-      generalize (inject_implies_image_in _ _ _ INJ23).
-      intros IMGIN23.
-      generalize (inject_implies_dom_in _ _ _ INJ12).
-      intros DOMIN12.
-      generalize (inject_implies_dom_in _ _ _ INJ23).
-      intros DOMIN23.
-      generalize (inject_implies_dom_in _ _ _ INJ13').
-      intros DOMIN13'.
-      generalize (Mem.unchanged_on_support _ _ _ UNCHANGE1).
-      intros SUPINCL1.
-      generalize (Mem.unchanged_on_support _ _ _ UNCHANGE3).
-      intros SUPINCL3.
-      generalize (inject_incr_inv _ _ _ _ _ _ _ DOMIN12 IMGIN12 DOMIN23 DOMIN13' SUPINCL1 INCR13 DISJ13).
-      intros (j12' & j23' & m2'_sup & JEQ & INCR12 & INCR23 & SUPINCL2 & DOMIN12' & IMGIN12' & DOMIN23' & INCRDISJ12 & INCRDISJ23 & INCRNOLAP & ADDZERO & ADDEXISTS & ADDSAME).
-      subst. cbn in *.
-      set (m2'A := m2' m1A m2A m1'A j12 j23 j12' m2'_sup INJ12 ).
-      assert (INJ12' :  Mem.inject j12' m1'A m2'A). eapply INJ12'; eauto.
-      assert (INJ23' :  Mem.inject j23' m2'A m3'A). eapply INJ23'; eauto.
-      set (w12' := injpw j12' m1'A m2'A INJ12').
-      set (w23' := injpw j23' m2'A m3'A INJ23').
-      rename vres2 into vres3.
-      exploit compose_meminj_midvalue; eauto.
-      intros [vres2 [RES1 RES2]].
-      assert (UNC21:Mem.unchanged_on (loc_out_of_reach j12 m1A) m2A m2'A).
-      eapply UNCHANGE21; eauto.
-      (* end of injp decomposition *)
-      set (r2 := cr vres2 m2'A ).
-      edestruct Hk12 as (i12' & s2' & Hs2' & Hs12'); eauto.
-      instantiate (1:= r2).
-      exists w12'. split. constructor; eauto. eapply ROUNC2; eauto.
-      eapply MAXPERM2; eauto.
-      eapply Mem.unchanged_on_implies; eauto.
-      intros. red. unfold compose_meminj.
-      rewrite H7. reflexivity.
-      constructor; eauto. constructor; eauto.
-      edestruct Hk23 as (i23' & s3' & Hs3' & Hs23'); eauto.
-      instantiate (1:= (cr vres3 m3'A)). exists w23'.
-      split. constructor; eauto. eapply ROUNC2; eauto.
-      eapply MAXPERM2; eauto.
-      eapply UNCHANGE22; eauto. eapply out_of_reach_trans; eauto.
-      constructor; eauto. constructor.
-      exists (i23', i12'), s3'. split; auto. exists s2', w12, w23; intuition eauto.
-      
-  }
-- (* simulation *)
-  intros. destruct H0 as (s3 & w12 & w23 & MS1 & MS2 & MENV1 & MENV2 & RESULT).
-  destruct i as [i2 i1]; simpl in *.
-  edestruct (@fsim_simulation') as [(i1' & s3' & C & D) | (i1' & C & D & E)]; eauto.
-+ (* L2 makes one or several steps. *)
-  edestruct (@simulation_plus') as [(i2' & s2' & P & Q) | (i2' & P & Q & R)]; eauto.
-* (* L3 makes one or several steps *)
-  exists (i2', i1'); exists s2'; split. auto. exists s3', w12, w23; auto.
-* (* L3 makes no step *)
-  exists (i2', i1'); exists s2; split.
-  right; split. subst t; apply star_refl. red. left. auto.
-  exists s3', w12, w23; auto.
-+ (* L2 makes no step *)
-  exists (i2, i1'); exists s2; split.
-  right; split. subst t; apply star_refl. red. right. auto.
-  exists s3, w12, w23; auto.
+        edestruct H30; eauto.
+    + constructor; cbn; eauto with mem.
+      eapply Values.val_inject_compose; eauto.
 Admitted.
 
-(*
-Lemma compose_fsim_components':
-  fsim_components' (cc_c' injp') (cc_c' injp') L1 L2 ->
-  fsim_components' (cc_c' injp') (cc_c' injp') L2 L3 ->
-  fsim_components' (cc_c' injp') (cc_c' injp') L1 L3.
+Theorem injp'_injp_ref2:
+  ccref' (cc_compose_2 (cc_c' injp') (cc_c injp)) (cc_c' injp') .
 Proof.
-  intros [index order match_states Hsk props order_wf].
-  intros [index' order' match_states' Hsk' props' order_wf'].
-  set (ff_index := (index' * index)%type).
-  set (ff_order := lex_ord (clos_trans _ order') order).
-  set (ff_match_states :=
-         fun se1 se3 (w: injp_world) (i: ff_index) (s1: state L1) (s3: state L3) =>
-           exists s2,
-             match_states se1 se1 (id_world w) (snd i) s1 s2 /\
-             match_states' se1 se3 w (fst i) s2 s3).
-  apply Forward_simulation' with ff_order ff_match_states.
-  3: { unfold ff_order. auto using wf_lex_ord, wf_clos_trans. }
-  1: { etransitivity; eauto. }
-  intros se1 se2 w Hse2 Hcompat. cbn in *.
-  assert (Hse1: injp_match_stbls' (id_world w) se1 se1).
-  { clear - Hse2.
-    inv Hse2. constructor; eauto.
-    inv H. constructor; intros; eauto.
-    - unfold meminj_dom in H2. destruct (f b1); try discriminate
-    
-  }
-  assert (Hse1: Genv.valid_for (skel L1) se1).
-  {}
-  { rewrite <- Hsk. eapply match_senv_valid_for; eauto. }
-  constructor.
-- (* valid query *)
-  intros q1 q3 (q2 & Hq12 & Hq23).
-  erewrite fsim_match_valid_query by eauto.
-  eapply fsim_match_valid_query; eauto.
-- (* initial states *)
-  intros q1 q3 s1 (q2 & Hq12 & Hq23) Hs1.
-  edestruct (@fsim_match_initial_states liA1) as (i & s2 & A & B); eauto.
-  edestruct (@fsim_match_initial_states liA2) as (i' & s3 & C & D); eauto.
-  exists (i', i); exists s3; split; auto. exists s2; auto.
-- (* final states *)
-  intros. cbn. destruct H as (s3 & A & B).
-  edestruct (@fsim_match_final_states liA1) as (r2 & Hr2 & Hr12); eauto.
-  edestruct (@fsim_match_final_states liA2) as (r3 & Hr3 & Hr23); eauto.
-- (* external states *)
-  intros. destruct H as [s3 [A B]].
-  edestruct (@fsim_match_external liA1) as (w12 & q2 & Hq2 & Hq12 & Hw12 & Hk12); eauto.
-  edestruct (@fsim_match_external liA2) as (w23 & q3 & Hq3 & Hq23 & Hw23 & Hk23); eauto.
-  exists (se2, w12, w23), q3. cbn; repeat apply conj; eauto.
-  intros r1 r3 s1' (r2 & Hr12 & Hr23) Hs1'.
-  edestruct Hk12 as (i12' & s2' & Hs2' & Hs12'); eauto.
-  edestruct Hk23 as (i23' & s3' & Hs3' & Hs23'); eauto.
-  exists (i23', i12'), s3'. split; auto. exists s2'; auto.
-- (* simulation *)
-  intros. destruct H0 as [s3 [A B]]. destruct i as [i2 i1]; simpl in *.
-  edestruct (@fsim_simulation' liA1) as [(i1' & s3' & C & D) | (i1' & C & D & E)]; eauto.
-+ (* L2 makes one or several steps. *)
-  edestruct (@simulation_plus liA2) as [(i2' & s2' & P & Q) | (i2' & P & Q & R)]; eauto.
-* (* L3 makes one or several steps *)
-  exists (i2', i1'); exists s2'; split. auto. exists s3'; auto.
-* (* L3 makes no step *)
-  exists (i2', i1'); exists s2; split.
-  right; split. subst t; apply star_refl. red. left. auto.
-  exists s3'; auto.
-+ (* L2 makes no step *)
-  exists (i2, i1'); exists s2; split.
-  right; split. subst t; apply star_refl. red. right. auto.
-  exists s3; auto.
-Qed.
-*)
-Lemma compose_forward_simulations_old_new:
-  forward_simulation (cc_c injp) (cc_c injp) L1 L2 ->
-  forward_simulation' (cc_c' injp') (cc_c' injp') L2 L3 ->
-  forward_simulation' (cc_c' injp') (cc_c' injp') L1 L3.
-Proof.
-  intros [X] [Y]. constructor.
-  apply compose_fsim_components_old_new; auto.
-Qed.
+  red.
+  intros w se1 se3 q1 q3 MSTBL13 MMEM13.
+  destruct w as [[se2 w12] w23].
+  destruct MSTBL13 as [MSTBL12 MSTBL23].
+  destruct MMEM13 as [q2 [MMEM12 MMEM23]].
+  inv MMEM12. inv H1. rename f into j12. rename Hm0 into INJ12. clear Hm1.
+  inv MMEM23. inv H9. rename f into j23. rename Hm1 into INJ23. clear Hm2.
+  cbn in H8, H6, MSTBL23, MSTBL12, H, H0.
+  assert (gs0 = gs2).
+  inv MSTBL12. inv MSTBL23. eauto. subst gs0.                
+  exists ((injpw (compose_meminj j12 j23) gs1 gs3
+          m1 m3 (Mem.inject_compose _ _ _ _ _ INJ12 INJ23))).
+  simpl. repeat apply conj.
+  - inv MSTBL12. inv MSTBL23.
+    econstructor; simpl; auto.
+    eapply Genv.match_stbls_stbls'_compose; eauto.
+    eapply Genv.match_stbls_compose; eauto.
+  red. intros w se1 se2 q1 q2 Hse Hq.
+  inv Hse. inv Hq. cbn in H2, H3. inv H4. rename m0 into m1. rename m3 into m2.
+  exists (se1, (injpw (meminj_dom f) (Genv.genv_sup se1) (Genv.genv_sup se1) m1 m1 (mem_inject_dom f m1 m2 Hm)),
+      (injpw f (Genv.genv_sup se1) (Genv.genv_sup se2) m1 m2 Hm)).
 
-End COMPOSE_FORWARD_SIMULATIONS.
-*)
+  
+
+Theorem injp'_injp_c_equiv:
+  cceqv' (cc_c' injp') (cc_compose_2 (cc_c' injp') (cc_c injp)).
+Admitted.
+
+(** * hard part : compose injp ⋅ injp' ≡ injp' *)
+  
+(** We need a refinement at top-level *)
+Theorem refinement_injp_injp'_c:
+  cceqv' (cc_c' injp') (cc_compose_1 (cc_c injp) (cc_c' injp')).
+Abort.
+
+
+
+
